# Chemical Equilibrium 
> Date: 16/8/25

| S. No. | Reversible Reaction | Irreversible reaction | 
|:-:|:-:|:-:|
| 1. | Can go in both forward and backward direction. | Reaction can only go forward | 
| 2. | Chemical equilibrium can only be obtained in reversible reaction | Equilibrium cannot be obtained here | 
| 3. | E.g.: $N_2 + 3H_2 \leftrightarrows 2NH_3$ | E.g.: $AgNO_3 + NaCl \rightarrow AgCl + Na$ | 
| 4. | $\leftrightarrows$ is compulsory for reversible reaction. | $\rightarrow$ should be given for Irreversible reaction. | 
| 5. | Equilibrium can only be obtained in a closed vessel. | Closed vessel isn't required for this reaction. | 

- $\underset{50}{A} + \underset{50}{B} \leftrightarrows \underset{50}{C} + \underset{50}{D}$


## Characteristics of Chemical Equilibrium 
1. An Equilibrium is attained only in a closed vessel in a certain temperature. Eg: $CaCO_3 \leftrightarrows CaO + CO_2 (\uparrow)$, since $CO_2$ will escape if container is open, and the equation will no longer be reversible. 
2. Chemical Equilibrium can be attained from both directions, i.e., forward and backward. 
3. Rate of forward reaction is equal to the rate of backwarrd reaction in reversible reaction, i.e., chemical equilibrium. Eg: $CaCO_3 \overset{R_f}{\underset{R_b}{\leftrightarrows}} CaO + CO_2 (\uparrow)$
4. Chemical equilibrium is **dynamic** in nature. Because buring reaction, the concentration of rate of reactants decrease and that of product increases till the equilibrium is attained.
5. At equilibrium, it appears that the reaction has stopped but practically, the reaction is still occuring with same rate of forward and backward direction. 
6. A catalyst has no effect on the state of equilibrium. It normally increases the rate of both forward and backward reaction. It helps to **attain equilibrium quickly to same extent**. 

- **Catalyst:** it is a substance that can increase or decrease the rate of reaction without being consumed in the reaction. 


$$
\text{Concentration} = \frac{\text{No. of Moles}(n)}{\text{Volume}(V)} 
$$

## Laws of Mass Action 
$$
\underset{\text{Reactant}}{A+B} \leftrightarrows \underset{\text{Product}}{C+D}
$$ 

A Mixture of reactants and products in equilibrium state are known as **equilibrium mixture**. 

- It states that the rate of chemical reaction is directly proportional to the multiplication product of active masses at **constant temperature**.

$$
R_f \propto [A][B] \implies R_f = K_f [A][B]
\\ 
R_b \propto [C][D] \implies R_b = K_b [C][D]
$$

According to equation, 

$R_f = R_b$  
$\implies K_f [A][B] = K_b [C][D]$  
$\implies \frac{K_f}{K_b} = \frac{[C][D]}{[A][B]}$  
$\implies K_c = \frac{[C][D]}{[A][B]}$  

$$
aA + bB \overset{R_f}{\underset{R_b}{\leftrightarrows}} cC + dD 
$$

For reactions having stoichiometric coefficient, 

$$
\text{Rate of reaction} \propto \text{Multiplication of concentration raised to power of their coefficients}
$$

$R_f \propto [A]^a[B]^b = K_f [A]^a[B]^b$  
$R_b \propto [C]^c[D]^d = K_b [C]^c[D]^d$  
$\implies \frac{K_f}{K_b} = \frac{[C]^c[D]^d}{[A]^a[B]^b}$  
$\implies K_C = \frac{[C]^c[D]^d}{[A]^a[B]^b}$


- Equilibrium constant is the ratio of multiplication of concentration of products by that of reactants raised to the power of their stoichiometric coefficients. 

$PV = nRT$

- **P**: Pressure 
- **V**: Volume 
- **n**: No. of moles 
- **R**: Gas constant
- **T**: Temperature 

$P = \frac{nRT}{V}$  
$P = CRT$  
$P \propto C$

$aA + bB \leftrightarrows cC + dD$
$K_p = \frac{P_C^c P_D^d}{P_A^a P_B^b}$

$4NH_3 + 5O_2 \leftrightarrows 4NO + 6H_2O$

$K_C = \frac{[NO]^4[H_2O]^6}{[NH_3]^4[O_2]^5}$  
$K_P = \frac{[P_{NO}]^4[P_{H_2O}]^6}{[P_{NH_3}]^4[P_{O_2}]^5}$

$aA + bB \leftrightarrows cC + dD$

$P = CRT$

- $P_A = [A]RT$
- $P_B = [B]RT$
- $P_C = [C]RT$
- $P_D = [D]RT$

$K_P = \frac{P_C^c P_D^d}{P_A^a P_B^b}$  
$\implies \frac{ {[C]RT}^C {[D]RT}^d } { {[A]RT^a} {[B]RT}^b }$  
$\implies \frac{[C]^c [D]^d}{[A]^a [B]^b}$  
$\implies \frac{(RT)^{c+d}}{(RT)^{a+b}}$  
$\implies K_C = (RT)^{(c+d)-(a+b)}$  
$\K_p = K_C (RT)^{\Delta ng}$  
$\Delta ng = (c+d)-(a+b)$

$2 A(g) = B(g) + C (g)$  
$A ng = (1+1)-2$  
$A = 0$
$K_P = K_C (RT)^{\Delta ng}$  
$\implies K_C (RT)^0$  
$K_P = K_C \times 1$
$\therefore K_P = K_C$
